%!TEX root=fp-intro.tex

\section{The $\lambda$-Calculus}

%
\begin{frame}{The untyped $\lambda$-calculus}

The $\lambda$-calculus is the formalism that underlies the functional approach
to programming.

The simplest version is the \textbf{untyped $\lambda$-calculus}, or simply
$\lambda$.

The $lambda$-calculus is a \textbf{core language} for many functional languages.
Convenient language structures can be defined by translation into $\lambda$.

Haskell actually uses a typed variant called \textbf{System F}, but the
principles are the same.

\end{frame}

%
\begin{frame}{The $\lambda$-calculus}

The grammar for the language is extremely simple.

\begin{block}{Grammar for the simple untyped $\lambda$-calculus}
\begin{tabular}{lll}
  $e$ \texttt{::=} & $x$              & \emph{(variable)} \\
                   & $e_1 \; e_2$     & \emph{(application)} \\
                   & $\lambda x . e$  & \emph{(abstraction)} \\
\end{tabular}
\end{block}

We may also use parentheses to disambiguate expressions.

\end{frame}

%
\begin{frame}{Semantics}

The only means to ``compute'' in this language is to apply functions to
arguments (which are themselves functions). For example, we can define the
identity function, which just returns its argument:

\begin{block}{Identity function}
\[
\mathtt{id} = \lambda x . x
\]
\end{block}

\end{frame}

%
\begin{frame}{Semantics}

Given an expression in the $\lambda$-calculus, we can \textbf{evaluate} it by
manipulating expressions according to the rules of some \textbf{operational
semantics}.

The most popular operational semantics are \textbf{call-by-value}.

Haskell's semantics are based on a very different semantics --
\textbf{call-by-need}.

\end{frame}

%
\begin{frame}{Notation}

Operational semantics have their own idiosyncratic notation.

\begin{columns}[t]
\begin{column}{0.5\textwidth}

\begin{block}{Conditions}
Read $\infer{c}{a \; b}$ as ``if $a$ and $b$, then $c$''.
\end{block}

\begin{block}{Transitions}
Read $a \to b$ as ``$a$ rewrites to $b$''.
\end{block}

\end{column}
\begin{column}{0.4\textwidth}

\begin{block}{Renaming}
Read $[x \mapsto a] b$ as ``$x$ is rewritten to $a$ wherever $x$ occurs in the 
expression $b$''.
\end{block}

\end{column}
\end{columns}

\end{frame}


%
\begin{frame}{Call-by-value}

\begin{columns}
\begin{column}{0.4\textwidth}

\begin{block}{Expressions}
\begin{tabular}{ll}
$e$ \texttt{::=} & $x$              \\
                 & $e \; e$         \\
                 & $\lambda x . e$  \\
\end{tabular}
\end{block}

\begin{block}{Values}
\begin{tabular}{ll}
$v$ \texttt{::=} & $\lambda x . e$  \\
\end{tabular}
\end{block}

\end{column}
\begin{column}{0.4\textwidth}

\begin{block}{Evaluation}
\[
\infer{e_1 e_2 \to e_1' e_2}{e_1 \to e_1'}
\]
\[
\infer{v_1 e_2 \to v_1' e_2}{e_2 \to e_2'}
\]
\[
\infer{(\lambda x . e) v \to \left[x \mapsto v \right] \, e}{}
\]
\end{block}

\end{column}
\end{columns}

\end{frame}

%
\begin{frame}{Call-by-need}

\begin{columns}
\begin{column}{0.4\textwidth}

\begin{block}{Expressions}
\begin{tabular}{ll}
$e$ \texttt{::=} & $x$              \\
                 & $e \; e$         \\
                 & $\lambda x . e$  \\
\end{tabular}
\end{block}

\begin{block}{Values}
\begin{tabular}{ll}
$v$ \texttt{::=} & $\lambda x . e$  \\
\end{tabular}
\end{block}

\end{column}
\begin{column}{0.4\textwidth}

\begin{block}{Evaluation}
\[
\infer{e_1 e_2 \to e_1' e_2}{e_1 \to e_1'}
\]
\[
\infer{(\lambda x . e_1) e_2 \to \left[x \mapsto e_2 \right] \, e_1}{}
\]
\end{block}

\end{column}
\end{columns}

\end{frame}

%
\begin{frame}{Extensions}

We can extend the untyped $\lambda$-calculus with natural numbers and simple
arithmetic -- makes examples easier to grok.

We also introduce a \texttt{let} syntactic sugar:

\begin{block}{\texttt{let} expressions}
Define

\[
\mathtt{let} \; x \; \mathtt{=} \; e_1 \; \mathtt{in} \; e_2
\]

to mean

\[
(\lambda x . e_2) \; e_1
\]
\end{block}

\end{frame}

%
\begin{frame}[fragile]{Example}

\begin{block}{}
\begin{verbatim}
let f = \x -> x + x in f (1 + 2)
\end{verbatim}
\end{block}

\begin{block}{Evaluation (call-by-value)}
\begin{verbatim}
   (\f -> f (1 + 2)) (\x -> x + x)
=> (\x -> x + x) (1 + 2)
=> (\x -> x + x) 3
=> 3 + 3
=> 6
\end{verbatim}
\end{block}

\begin{block}{Evaluation (call-by-need)}
\begin{verbatim}
   (\f -> f (1 + 2)) (\x -> x + 5)
=> (\x -> x + x) (1 + 2)
=> (1 + 2) + (1 + 2)
=> ...
=> 6
\end{verbatim}
\end{block}


\end{frame}

% %
% \begin{frame}{Scope}
% 
% Dynamic vs. static
% 
% \end{frame}

%
\begin{frame}{Recursion}

It may seem like complicated control flow would be difficult or impossible in
the untyped $\lambda$-calculus.

Not true -- we can use \textbf{fixpoint combinators} to define general recursive
functions. Therefore, the untyped $\lambda$-calculus is Turing complete!

Recall that a \textbf{fixed point} of a function $f$ is a value $x$ such that
$f(x) = x$.

\end{frame}

%
\begin{frame}{Y-combinator}

The \textbf{Y-combinator} is a famous fixpoint combinator.

\begin{block}{Y-combinator}
$Y = \lambda f.(\lambda x.f (x \; x)) (\lambda x.f (x \; x))$
\end{block}

In fact, there are infinitely many such combinators.

\end{frame}

%
\begin{frame}[fragile]{Recursion}

We can use a fixpoint combinator to essentially generate new copies of a
function body, as needed. This gives us recursion.

\begin{block}{Factorial function}
\begin{verbatim}
let fix = \f -> (\x -> f (x x)) (\x -> f (x x)) in 
let fact = 
  fix (\g -> (\n -> if n = 0 then 1 else n * (g (n - 1)))) 
in
fact 5
-- fact 5 => 120
\end{verbatim}
\end{block}

It isn't very important (nor easy!) to understand precisely \emph{how} this
works. Just remember that this gives us a formal basis for recursion.

\end{frame}
